soundness and completeness of reduction semantics
I formulated the reduction semantics as a relation (which is fitting but
also simplifies the proof). I had to correct the semantics in one little
detail.

Coq/Contracts.v
@@ -76,15 +76,6 @@ Definition obs := inp Z.
 
 Definition choices := inp bool.
 
-Definition plusZnat (n : nat) (z : Z) : Z := (Z_of_nat n + z)%Z.
-
-Infix "+#" := plusZnat (at level 60, right associativity).
-
-Lemma plusZnat_assoc z n m : n +# m +# z = (n + m +# z). 
-Proof.
-  unfold "+#". rewrite -> Z.add_assoc. rewrite <- Nat2Z.inj_add. reflexivity.
-Qed.
-
 
 Class Partial t := {
   lep : t -> t -> Prop
@@ -118,33 +109,34 @@ Instance nested_Partial T1 T2 (p1:Partial T1) (p2 : Partial T2) : Partial (T1 * 
 
 (* Move observations into the future. *)
 
-Definition adv_inp {A} (d : nat) (e : inp A) : inp A
-  := fun x => e (d +# x).
+Definition adv_inp {A} (d : Z) (e : inp A) : inp A
+  := fun x => e (d + x)%Z.
 
 Lemma adv_inp_0 A (e : inp A) : adv_inp 0 e = e.
 Proof.
   apply functional_extensionality.
-  unfold adv_inp. unfold "+#". rewrite Nat2Z.inj_0. reflexivity.
+  unfold adv_inp. reflexivity.
 Qed.
 
 Lemma adv_inp_iter {A} d d' (e : inp A) : adv_inp d (adv_inp d' e) = adv_inp (d' + d) e.
 Proof.
   apply functional_extensionality. induction d'; intros.
-  simpl. rewrite adv_inp_0. reflexivity.
-  simpl. unfold adv_inp in *.  rewrite plusZnat_assoc. reflexivity.
+  - simpl. rewrite adv_inp_0. reflexivity.
+  - simpl. unfold adv_inp in *.  rewrite Z.add_assoc. reflexivity.
+  - unfold adv_inp. rewrite Z.add_assoc.  reflexivity.
 Qed.
 
 
 Lemma adv_inp_swap {A} d d' (e : inp A) : 
   adv_inp d (adv_inp d' e) = adv_inp d' (adv_inp d e).
 Proof.
-  repeat rewrite adv_inp_iter. rewrite plus_comm. reflexivity.
+  repeat rewrite adv_inp_iter. rewrite Z.add_comm. reflexivity.
 Qed.
 
 
 Definition env := (obs * choices)%type.
 
-Definition adv_env (d : nat) (rho : env) : env :=
+Definition adv_env (d : Z) (rho : env) : env :=
   let (obs, ch) := rho in (adv_inp d obs, adv_inp d ch).
                                              
 
@@ -248,15 +240,16 @@ Definition trans := party -> party -> currency -> Z.
 Definition transfers := option trans.
 
 
-
-Definition empty_trans : transfers := Some (fun p1 p2 c => 0%Z).
+Definition empty_trans' : trans := fun p1 p2 c => 0%Z.
+Definition empty_trans : transfers := Some empty_trans'.
 Definition bot_trans : transfers := None.
-Definition singleton_trans p1 p2 c r : transfers 
-  := Some (fun p1' p2' c' => if andb (eq_str p1 p1') (andb (eq_str p2 p2') (eq_str c c')) then r else 0%Z).
-Definition add_trans : transfers -> transfers -> transfers
-  := option_map2 (fun t1 t2 p1 p2 c => (t1 p1 p2 c + t2 p1 p2 c)%Z).
-Definition scale_trans : option Z -> transfers -> transfers 
-  := option_map2 (fun s t p1 p2 c => (t p1 p2 c * s)%Z).
+Definition singleton_trans' p1 p2 c r : trans 
+  := fun p1' p2' c' => if andb (eq_str p1 p1') (andb (eq_str p2 p2') (eq_str c c')) then r else 0%Z.
+Definition singleton_trans p1 p2 c r : transfers  := Some (singleton_trans' p1 p2 c r).
+Definition add_trans' : trans -> trans -> trans := fun t1 t2 p1 p2 c => (t1 p1 p2 c + t2 p1 p2 c)%Z.
+Definition add_trans : transfers -> transfers -> transfers := option_map2 add_trans'.
+Definition scale_trans' : Z -> trans -> trans := fun s t p1 p2 c => (t p1 p2 c * s)%Z.
+Definition scale_trans : option Z -> transfers -> transfers := option_map2 scale_trans'.
 
 (* Traces represent the sequence of obligations that a contract
 specifies. *)
@@ -338,7 +331,7 @@ Fixpoint Csem (c : contract) : env -> trace :=
       | Zero => empty_trace
       | TransfOne p1 p2 c => singleton_trace (singleton_trans p1 p2 c  1)
       | Scale e c' => scale_trace R[|e|](fst rho) (C[|c'|]rho) 
-      | Transl d c' => (delay_trace d) (C[|c'|](adv_env d rho))
+      | Transl d c' => (delay_trace d) (C[|c'|](adv_env (Z.of_nat d) rho))
       | Both c1 c2 => add_trace (C[|c1|]rho) (C[|c2|]rho)
       | IfWithin e d c1 c2 => within_sem C[|c1|] C[|c2|] e rho d
     end
@@ -375,7 +368,7 @@ Qed.
 
 Lemma adv_inp_monotone A (in1 in2 : inp A) n : in1 ⊆ in2 -> adv_inp n in1 ⊆ adv_inp n in2.
 Proof. 
-  unfold lep, adv_inp. simpl. intros. remember (in1 (n +# i) j) as X.
+  unfold lep, adv_inp. simpl. intros. remember (in1 (n + i)%Z j) as X.
   destruct X;tryfalse. apply H. rewrite <- H0. auto. 
 Qed.
 
@@ -399,7 +392,7 @@ Proof.
     pose (IHc _ _ S i) as IHi. 
     destruct X; tryfalse. rewrite <- HeqX in * by auto. erewrite IHi by auto.
     auto.
-  - simpl. apply adv_env_monotone with (n := n) in S. apply IHc in S.
+  - simpl. apply adv_env_monotone with (n := Z.of_nat n) in S. apply IHc in S.
     simpl in S. unfold delay_trace in *. destruct (leb n i); auto.
   - unfold add_trace, add_trans in *. 
     remember (C[|c1|] rho1 i) as X1. remember (C[|c2|] rho1 i) as X2.
@@ -428,92 +421,115 @@ Qed.
 
 (********** Reduction semantics **********)
 
-Fixpoint adv_rexp (d : nat) (e : rexp) : rexp :=
+Fixpoint adv_rexp (d : Z) (e : rexp) : rexp :=
   match e with
     | RLit r => RLit r
     | RBin op e1 e2 => RBin op (adv_rexp d e1) (adv_rexp d e2)
     | RNeg e' => RNeg (adv_rexp d e')
-    | Obs o i => Obs o (d +# i)
+    | Obs o i => Obs o (d + i)%Z
   end.
 
-Fixpoint adv_bexp (d : nat) (e : bexp) : bexp :=
+Fixpoint adv_bexp (d : Z) (e : bexp) : bexp :=
   match e with
     | BLit b => BLit b
-    | BChoice c i => BChoice c (d +# i)
+    | BChoice c i => BChoice c (d + i)
     | BOp op e1 e2 => BOp op (adv_bexp d e1) (adv_bexp d e2)
     | RCmp op e1 e2 => RCmp op (adv_rexp d e1) (adv_rexp d e2)
     | BNot e' => BNot (adv_bexp d e')
   end.
 
 
-Fixpoint red' (rho : env) (c : contract) : option (contract * transfers) :=
-  match c with
-     | Zero => Some (Zero , None)
-     | TransfOne c p1 p2 => Some (Zero, singleton_trans c p1 p2 1)
-     | Scale e c1 => match red' rho c1 with
-                       | Some (c',t) => match t with
-                          | Some t' => match R[| e |] (fst rho) with
-                            | Some v => Some (Scale (adv_rexp 1 e) c', Some (fun p1 p2 c => (t' p1 p2 c * v)%Z))
-                            | None  => None
-                                       end
-                          | None => Some (Scale (adv_rexp 1 e) c', None)
-                                        end
-                       | _ => None 
-                     end
-     | Transl n c1 => match n with
-                          | 0 => red' rho c1
-                          | S n' => Some (Transl n' c1, None)
-                      end
-     | Both c1 c2 => match red' rho c1, red' rho c2 with
-                        | Some (c1', t1), Some (c2', t2) => 
-                          let t := match t1, t2 with
-                                    | None, None => None
-                                    | None, Some t2' => Some t2'
-                                    | Some t1', None => Some t1'
-                                    | Some t1', Some t2' => Some (fun p1 p2 c => t1' p1 p2 c + t2' p1 p2 c)%Z
-                                  end
-                          in Some (Both c1' c2', t)
-                        | _, _ => None
-                     end
-     | IfWithin b n c1 c2 => match B[|b|] rho with
-                               | None => None
-                               | Some true => red' rho c1
-                               | Some false => match n with
-                                                | 0 => red' rho c2
-                                                | S n => Some (IfWithin b n c1 c2, None)
-                                               end
-                             end
-  end.
+Inductive Red : contract -> env -> contract -> trans -> Prop :=
+| red_zero rho : Red Zero rho Zero empty_trans'
+| red_transf c p1 p2 rho : Red (TransfOne c p1 p2) rho Zero (singleton_trans' c p1 p2 1)
+| red_scale e rho c c' t v :  R[| e |] (fst rho) = Some v -> Red c rho c' t ->
+               Red (Scale e c) rho (Scale (adv_rexp (-1) e) c') (scale_trans' v t)
+| red_trans0 c rho c' t : Red c rho c' t -> Red (Transl 0 c) rho c' t
+| red_transS c rho n : Red (Transl (S n) c) rho (Transl n c) empty_trans'
+| red_both c1 c1' c2 c2' rho t1 t2 : Red c1 rho c1' t1 -> Red c2 rho c2' t2 -> 
+                         Red (Both c1 c2) rho (Both c1' c2') (add_trans' t1 t2)
+| red_if0_false rho c1 c2 c' b t : B[|b|] rho = Some false -> Red c2 rho c' t -> Red (IfWithin b 0 c1 c2) rho c' t
+| red_ifS_false rho c1 c2 n b : B[|b|] rho = Some false -> Red (IfWithin b (S n) c1 c2) rho (IfWithin b n c1 c2) empty_trans'
+| red_if_true rho c1 c2 c' n b t : B[|b|] rho = Some true -> Red c1 rho c' t -> Red (IfWithin b n c1 c2) rho c' t
+.
 
-Definition mk_empty_trans (t : transfers) : trans :=
-  match t with
-    | None => (fun p1 p2 c => 0)%Z
-    | Some t => t
-  end.
+Hint Constructors Red.
 
-Definition red (rho : env) (c : contract) : option (contract * trans) := 
-  match red' rho c with
-      | None => None
-      | Some (c, t) => Some (c, mk_empty_trans t)
-  end.
-
-Theorem red_complete c rho : red rho c = None -> C[|c|]rho 0 = None.
+Theorem red_sound1 c c' rho t  : Red c rho c' t ->  C[|c|]rho 0 = Some t.
 Proof.
-  unfold red. intro H. remember (red' rho c) as R. destruct R.
-  destruct p. destruct t. inversion H. inversion H. clear H.
-  induction c; simpl; try (inversion HeqR).
-  - destruct (red' rho c). destruct p. destruct t. destruct (R[|r|](fst rho)).
-    inversion H0. reflexivity. inversion H0. unfold scale_trace. unfold compose.
-    rewrite IHc by auto. unfold scale_trans. apply option_map2_none.
-  - destruct n; tryfalse. unfold delay_trace. simpl. rewrite adv_env_0. auto.
-  - destruct (red' rho c1). destruct p. destruct (red' rho c2). destruct p. inversion H0.
-    unfold add_trace. rewrite IHc2. apply option_map2_none. reflexivity.
-    unfold add_trace. rewrite IHc1; reflexivity.
-  - destruct n; simpl; unfold within_sem.
-    + destruct (B[|b|]rho). destruct b0; auto. reflexivity.
-    + destruct (B[|b|]rho). destruct b0. auto. inversion H0. reflexivity.
+  intro R. induction R; simpl. 
+  - reflexivity.
+  - reflexivity.
+  - unfold scale_trace, compose. rewrite IHR. rewrite H. reflexivity.
+  - unfold delay_trace. simpl. rewrite adv_env_0. 
+    assumption.
+  - unfold delay_trace. reflexivity.
+  - unfold add_trace. rewrite IHR1. rewrite IHR2. reflexivity.
+  - rewrite H. assumption.
+  - rewrite H. unfold delay_trace. reflexivity.
+  - destruct n; simpl; rewrite H; assumption.
 Qed.
-  
+
+
+Lemma adv_rexp_obs d e rho : R[|adv_rexp d e|]rho = R[|e|](adv_inp d rho).
+Proof.
+  induction e; simpl; first [reflexivity | f_equal; assumption].
+Qed.
+
+Lemma adv_rexp_env d e rho : R[|adv_rexp d e|](fst rho) = R[|e|](fst (adv_env d rho)).
+Proof.
+  destruct rho. simpl. apply adv_rexp_obs.
+Qed.
+
+Theorem red_sound2 c c' i rho t  : Red c rho c' t ->  C[|c|]rho (S i) = C[|c'|](adv_env 1 rho) i.
+Proof.
+  intros R. induction R; simpl.
+  - reflexivity.
+  - reflexivity.
+  - unfold scale_trace, compose. rewrite -> adv_rexp_env. rewrite adv_env_iter. simpl.
+    rewrite adv_env_0. rewrite IHR.  reflexivity.
+  - unfold delay_trace. rewrite adv_env_0. assumption.
+  - unfold delay_trace. simpl. rewrite adv_env_iter. 
+    assert (Z.pos (Pos.of_succ_nat n) = (1 + Z.of_nat n)%Z).
+    assert (1%Z = Z.of_nat 1) by reflexivity. rewrite H.
+    rewrite <- Nat2Z.inj_add. reflexivity.
+    rewrite H. reflexivity.
+  - unfold add_trace. rewrite IHR1. rewrite IHR2. reflexivity.
+  - rewrite H. assumption.
+  - unfold delay_trace. rewrite H. simpl. f_equal. omega.
+  - destruct n; simpl; rewrite H; assumption.
+Qed.
+
+Theorem red_complete c rho t : C[|c|]rho 0 = Some t -> exists c', Red c rho c' t.
+Proof.
+  generalize dependent t. induction c; simpl; intros.
+  - inversion H. eauto.
+  - inversion H. eauto.
+  - unfold scale_trace, compose in *.
+    remember (R[|r|](fst rho)) as R. destruct R; tryfalse.
+    remember (C[|c|] rho 0) as C. destruct C;tryfalse. inversion H. 
+    assert (exists c', Red c rho c' t0) as R by auto.
+    destruct R as [c'].
+    eexists. apply red_scale; auto. apply H0.
+  - unfold delay_trace in *. destruct n; simpl in *. 
+    + rewrite adv_env_0 in *. apply IHc in H. destruct H as [c'].
+      eexists. constructor. apply H.
+    + inversion H. eexists. constructor.
+  -  unfold add_trace in *.
+     destruct (C[|c1|] rho 0);tryfalse. destruct (C[|c2|] rho 0);tryfalse.
+     pose (IHc1 _ eq_refl) as IH1.  pose (IHc2 _ eq_refl) as IH2.
+     destruct IH1. destruct IH2. inversion H. 
+     eexists. constructor; eassumption.
+  - remember (B[|b|]rho) as B. destruct B as [b'| ]. 
+    + destruct b'.
+      * destruct n; simpl in *; rewrite <- HeqB in *;apply IHc1 in H;
+        destruct H; eexists; apply red_if_true; eauto. 
+      * destruct n; simpl in *;rewrite <- HeqB in *.
+        apply IHc2 in H. destruct H. eexists. apply red_if0_false; eauto.
+        unfold delay_trace in H. simpl in *. inversion H. eexists. constructor; auto.
+    + destruct n; simpl in *; rewrite <- HeqB in *; inversion H.
+Qed.
+      
 
 (********** Equivalence of contracts **********)
 
@@ -556,11 +572,6 @@ Proof.
 Qed.
 
 
-Lemma adv_rexp_obs d e rho : R[|adv_rexp d e|]rho = R[|e|](adv_inp d rho).
-Proof.
-  induction e; simpl; first [reflexivity | f_equal; assumption].
-Qed.
-
 Lemma adv_env_ch d rho : snd (adv_env d rho) = adv_inp d (snd rho).
 Proof.
   unfold adv_env. destruct rho. reflexivity.
@@ -588,16 +599,16 @@ Proof.
 Qed.
 
 Theorem transl_ifwithin e d t c1 c2 : 
-  IfWithin (adv_bexp d e) t (Transl d c1) (Transl d c2) ⊑
+  IfWithin (adv_bexp (Z.of_nat d) e) t (Transl d c1) (Transl d c2) ⊑
   Transl d (IfWithin e t c1 c2).
 Proof.
   unfold lequiv, lep. simpl. induction t; intros.
-  simpl in *. rewrite adv_bexp_env in *. remember (B[|e|](adv_env d rho)) as b.
+  simpl in *. rewrite adv_bexp_env in *. remember (B[|e|](adv_env (Z.of_nat d) rho)) as b.
   destruct b. destruct b;  assumption. 
   unfold const_trace, bot_trans in H. inversion H.
 
   simpl in *.  rewrite adv_bexp_env in *. 
-  remember (B[|e|](adv_env d rho)) as b. repeat destruct b. assumption. 
+  remember (B[|e|](adv_env (Z.of_nat d) rho)) as b. repeat destruct b. assumption. 
   rewrite adv_env_swap. rewrite delay_trace_swap. 
   unfold delay_trace at 1.
   unfold delay_trace at 1 in H. 
@@ -633,20 +644,20 @@ Qed.
 
 
 Theorem transl_ifwithin_wequiv e d t c1 c2 : 
-  IfWithin (adv_bexp d e) t (Transl d c1) (Transl d c2) ≃
+  IfWithin (adv_bexp (Z.of_nat d) e) t (Transl d c1) (Transl d c2) ≃
   Transl d (IfWithin e t c1 c2). 
 Proof.
   unfold wequiv. intros. destruct H. apply lequiv_total. apply transl_ifwithin. assumption.
   
   
   unfold lequiv, lep. simpl. generalize dependent rho. induction t; intros.
-  simpl in *. rewrite adv_bexp_env in *. remember (B[|e|](adv_env d rho)) as b.
+  simpl in *. rewrite adv_bexp_env in *. remember (B[|e|](adv_env (Z.of_nat d) rho)) as b.
   destruct b. destruct b; reflexivity.
   unfold total in H. 
   contradiction (H d (bot_trans_delay_at d)). 
 
   simpl in *.  rewrite adv_bexp_env in *. 
-  remember (B[|e|](adv_env d rho)) as b. repeat destruct b. reflexivity.
+  remember (B[|e|](adv_env (Z.of_nat d) rho)) as b. repeat destruct b. reflexivity.
   rewrite adv_env_swap. rewrite delay_trace_swap. 
   rewrite IHt. reflexivity. rewrite delay_trace_swap in H. rewrite adv_env_swap.
   apply total_delay in H. assumption. apply bot_trans_delay_total in H. contradiction.
@@ -658,17 +669,17 @@ Qed.
 
 (* [obs_until d r1 r2] iff [r1] [r2] coincide at [d] and earlier. *)
 
-Definition inp_until {A} (d : nat) (r1 r2 : inp A) : Prop :=
-  forall z, Z.le z (Z.of_nat d) -> r1 z = r2 z.
+Definition inp_until {A} (d : Z) (r1 r2 : inp A) : Prop :=
+  forall z, Z.le z d -> r1 z = r2 z.
 
-Definition env_until (d : nat) (e1 e2 : env) : Prop :=
+Definition env_until (d : Z) (e1 e2 : env) : Prop :=
   inp_until d (fst e1) (fst e2) /\ inp_until d (snd e1) (snd e2).
 
 
 (* Semantic causality *)
 
 Definition causal (c : contract) : Prop :=
-  forall d r1 r2,  env_until d r1 r2 -> (C[|c|]r1) d = (C[|c|]r2) d.
+  forall d r1 r2,  env_until (Z.of_nat d) r1 r2 -> (C[|c|]r1) d = (C[|c|]r2) d.
 
 (* Provable causality *)
 
@@ -710,16 +721,15 @@ Lemma inp_until_adv {A} d t (r1 r2 : inp A):
 Proof.
   split.
   unfold inp_until in *. intros.
-  pose (H (z - Z.of_nat t)%Z) as H'.
-  unfold adv_inp in H'. unfold "+#" in H'.
-  assert (Z.of_nat t + (z - Z.of_nat t) = z)%Z as E by omega.
-  rewrite E in H'. apply H'.
-  rewrite Nat2Z.inj_add in H0. omega.
+  pose (H (z - t)%Z) as H'.
+  unfold adv_inp in H'. 
+  assert (t + (z - t) = z)%Z as E by omega.
+  rewrite E in H'. apply H'. omega.
 
   unfold inp_until in *. intros.
-  unfold adv_inp. unfold "+#".
+  unfold adv_inp. 
 
-  pose (H (Z.of_nat t + z)%Z) as H'.  apply H'. rewrite Nat2Z.inj_add. omega.
+  pose (H (t + z)%Z) as H'.  apply H'. omega.
 
 Qed.
 
@@ -730,7 +740,7 @@ Proof.
   repeat rewrite inp_until_adv. reflexivity.
 Qed.
 
-Lemma rpc_inp_until e d r1 r2 : R|-e -> inp_until d r1 r2 -> R[|e|]r1 = R[|e|]r2.
+Lemma rpc_inp_until e d r1 r2 : R|-e -> inp_until (Z.of_nat d) r1 r2 -> R[|e|]r1 = R[|e|]r2.
 Proof.
   intros R O. induction R; simpl; try (f_equal; assumption).
 
@@ -738,7 +748,7 @@ Proof.
   eapply Z.le_trans. apply H. apply Nat2Z.is_nonneg.
 Qed.
 
-Lemma bpc_env_until e d r1 r2 : B|-e -> env_until d r1 r2 -> B[|e|]r1 = B[|e|]r2.
+Lemma bpc_env_until e d r1 r2 : B|-e -> env_until (Z.of_nat d) r1 r2 -> B[|e|]r1 = B[|e|]r2.
 Proof.
   intros R O. destruct O. induction R; simpl; try (f_equal; assumption).
 
@@ -748,11 +758,11 @@ Proof.
   f_equal; eapply rpc_inp_until; eassumption.
 Qed.
 
-Lemma env_until_adv_1 d r1 r2 : 1 <= d -> env_until d r1 r2 ->
-                        env_until (d - 1) (adv_env 1 r1) (adv_env 1 r2).
+Lemma env_until_adv_1 d r1 r2 : (1 <= d -> env_until d r1 r2 ->
+                        env_until (d - 1) (adv_env 1 r1) (adv_env 1 r2))%Z.
 Proof.
   intros.
-  assert (1 + (d - 1) = d) by omega.
+  assert (1 + (d - 1) = d)%Z by omega.
   rewrite env_until_adv. rewrite H1. assumption.
 Qed.
 
@@ -764,7 +774,8 @@ Proof.
   unfold delay_trace.
   remember (leb d d0) as C. destruct C.
     symmetry in HeqC. apply leb_complete in HeqC.
-    apply IHpc. rewrite env_until_adv. assert (d + (d0 - d) = d0) as D by omega.
+    apply IHpc. rewrite env_until_adv. assert (Z.of_nat d + Z.of_nat(d0 - d) = Z.of_nat d0)%Z as D.
+    rewrite <- Nat2Z.inj_add. f_equal. omega.
     rewrite D. assumption.
     
     reflexivity.
@@ -788,8 +799,11 @@ reflexivity.
 
   erewrite bpc_env_until with (r2:=r2) by eassumption. 
   remember (B[|b|]r2) as bl. destruct bl. destruct b0.  eapply IHpc1; eassumption. 
-  unfold delay_trace. remember (leb 1 d) as L. destruct L.  apply IHl.
-  apply env_until_adv_1. apply leb_complete. auto. auto. reflexivity. reflexivity.
+  unfold delay_trace. remember (leb 1 d) as L. destruct L.  apply IHl. 
+  rewrite Nat2Z.inj_sub.
+  apply env_until_adv_1. symmetry in HeqL. apply leb_complete in HeqL. apply inj_le in HeqL. auto.
+  auto.
+  apply leb_complete. auto. auto. reflexivity. 
 Qed.
 
 
@@ -853,31 +867,32 @@ Inductive ppc : option nat -> contract -> Prop :=
                                      -> omin d1 (oplus l d2) ||-  IfWithin b l c1 c2
                                             where "d '||-' c" := (ppc d c). 
 
-Lemma inp_until_le {A} d1 d2 (r1 r2 : inp A) : d2 <= d1 -> inp_until d1 r1 r2 -> inp_until d2 r1 r2.
+Lemma inp_until_le {A} d1 d2 (r1 r2 : inp A) : Z.le d2 d1 -> inp_until d1 r1 r2 -> inp_until d2 r1 r2.
 Proof. 
-  unfold inp_until. intros. apply H0. apply inj_le in H. eapply Z.le_trans. apply H1. assumption.
+  unfold inp_until. intros. apply H0. omega.
 Qed.
 
-Ltac inp_until_max := eauto using inp_until_le, Max.le_max_l, Max.le_max_r.
+Ltac inp_until_max := eauto using inp_until_le, Z.le_max_l, Z.le_max_r.
 
-Lemma env_until_le d1 d2 r1 r2 : d2 <= d1 -> env_until d1 r1 r2 -> env_until d2 r1 r2.
+Lemma env_until_le d1 d2 r1 r2 : Z.le d2 d1 -> env_until d1 r1 r2 -> env_until d2 r1 r2.
 Proof. 
   unfold env_until. intros. destruct H0. split; eapply inp_until_le; eassumption.
 Qed.
 
-Ltac env_until_max := eauto using env_until_le, Max.le_max_l, Max.le_max_r.
+Ltac env_until_max := eauto using env_until_le, Z.le_max_l, Z.le_max_r.
 
-Lemma rppc_inp_until e d r1 r2 : d R||-e  -> inp_until d r1 r2 -> R[|e|]r1 = R[|e|]r2.
+Lemma rppc_inp_until e d r1 r2 : d R||-e  -> inp_until (Z.of_nat d) r1 r2 -> R[|e|]r1 = R[|e|]r2.
 Proof.
   intros R O. induction R; simpl; try solve [f_equal; auto].
 
   unfold inp_until in O. rewrite O. reflexivity. pose (Z_le_dec i 0%Z) as Z.
   destruct Z. eapply Z.le_trans. apply l. apply Zle_0_nat. rewrite Z2Nat.id; omega.
+  rewrite Nat2Z.inj_max in *.
 
   f_equal; first [apply IHR1|apply IHR2]; inp_until_max.
 Qed.
 
-Lemma bppc_env_until e d r1 r2 : d B||-e -> env_until d r1 r2 -> B[|e|]r1 = B[|e|]r2.
+Lemma bppc_env_until e d r1 r2 : d B||-e -> env_until (Z.of_nat d) r1 r2 -> B[|e|]r1 = B[|e|]r2.
 Proof.
   intros R O. induction R; simpl; try solve [f_equal; auto].
 
@@ -885,8 +900,9 @@ Proof.
   remember (0 <=? i)%Z as L. symmetry in HeqL. destruct L.
   rewrite <- Zle_is_le_bool in HeqL. rewrite Z2Nat.id; omega.
   rewrite Z.leb_gt in HeqL. pose (Zle_0_nat (Z.to_nat i)). omega.
-
+  rewrite Nat2Z.inj_max in *.
   destruct O. f_equal; eapply rppc_inp_until; inp_until_max.
+  rewrite Nat2Z.inj_max in *.
   f_equal; first [apply IHR1|apply IHR2]; env_until_max.
 Qed.
 
@@ -903,7 +919,7 @@ Qed.
 
 
 Definition wcausal (c : contract) : Prop :=
-  forall d r1 r2,  env_until d r1 r2 -> 
+  forall d r1 r2,  env_until (Z.of_nat d) r1 r2 -> 
                    (C[|c|]r1) d = None \/ (C[|c|]r2) d = None \/ (C[|c|]r1) d = (C[|c|]r2) d.
 
 Lemma rppc_indep' c r d N : N = None -> 
@@ -915,7 +931,7 @@ Proof.
   destruct b. inversion NN. 
   simpl. unfold delay_trace. remember (leb d d0) as L.
   destruct L. 
-  pose (IHppc NeN (d0 - d) (adv_env d r)) as IH. destruct IH; auto.
+  pose (IHppc NeN (d0 - d) (adv_env (Z.of_nat d) r)) as IH. destruct IH; auto.
   auto.
 
   inversion NN.
@@ -1018,7 +1034,8 @@ Proof.
   unfold delay_trace.
   remember (leb d d0) as C. destruct C.
     symmetry in HeqC. apply leb_complete in HeqC.
-    apply IHppc. rewrite env_until_adv. assert (d + (d0 - d) = d0) as D by omega.
+    apply IHppc. rewrite env_until_adv. assert (Z.of_nat d + Z.of_nat (d0 - d) = Z.of_nat d0)%Z as D.
+    rewrite <- Nat2Z.inj_add. f_equal. omega.
     rewrite D. assumption. auto.
     
     auto.
@@ -1027,7 +1044,7 @@ Proof.
   remember (R[|e|](fst r1)) as R1; remember (R[|e|](fst r2)) as R2; 
   destruct R1; destruct R2; try auto. 
   remember (leb d d0) as D. symmetry in HeqD. destruct D. rewrite leb_iff in HeqD.
-  inversion H2 as [H2' H2''].
+  inversion H2 as [H2' H2'']. apply inj_le in HeqD.
   pose (inp_until_le _ _ _ _ HeqD H2') as O.
   pose (IHppc _ _ _ H2) as IH. destruct IH. left.
   rewrite H3. reflexivity. destruct H3. right. left. rewrite H3.
@@ -1051,7 +1068,7 @@ Proof.
 
   auto.
 
-  assert (env_until 0 r1 r2). apply env_until_le with (d1:= d). omega. assumption.
+  assert (env_until 0 r1 r2). apply env_until_le with (d1:= Z.of_nat d). omega. assumption.
   generalize dependent d. generalize dependent r1. generalize dependent r2. 
   induction l; intros; simpl.
   
@@ -1064,6 +1081,7 @@ Proof.
   remember (B[|b|]r2) as bl. destruct bl. destruct b0.  eapply IHppc1; eassumption. 
   unfold delay_trace. remember (leb 1 d) as L. destruct L. 
   symmetry in HeqL. rewrite leb_iff in HeqL. apply IHl. apply env_until_adv. simpl.  
-  eapply env_until_le; eassumption. apply env_until_adv_1; assumption. auto. auto.
+  apply inj_le in HeqL. eapply env_until_le; eassumption. rewrite Nat2Z.inj_sub. apply env_until_adv_1.
+  apply inj_le in HeqL. assumption. auto. auto. auto. auto.
 Qed.
 
